ServiceProvider.fst
@@ -9,20 +9,26 @@ open Protocol
 
 val serviceprovider: me:prin -> client:prin -> idp:prin -> unit 
 let serviceprovider me client idp = 
+  
   let reqRes = recieve client in (*1*)
   match reqRes with
   | HttpGet (uri) -> 
+  
     let (authnReq, sigSP)  = CreateAuthnRequest me idp in 
-    assume(Log idp authnReq);
+    assume(Log idp "relay") (*Protocol event*);
+  
   	let authnReqest = SamlProtocolMessage idp authnReq sigSP "relay" in 
   	send client authnReqest; (*2*)
+  
   	let authResponse = recieve client in (*7*)
   	match authResponse with
   	| SamlProtocolMessage (sp, message, sigIDP, relay) -> 
+  
   		let resource = Resource uri in
   		send client resource	(*8*)
-  	| _ ->  send client (Failed (403))(*8.1*)     
-  | _ -> send client (Failed (400))(*2.1*)
   
+  	| _ ->  send client (Failed (403))(*8.1*)     
+  
+  | _ -> send client (Failed (400))(*2.1*)
 
 end (* Serviceprovider *)
