identityprovider.fst
@@ -9,25 +9,33 @@ open Protocol
 
 val identityprovider: me:prin -> client:prin -> sp:prin -> unit
 let identityprovider me client serviceprovider =
-	let authRequest = recieve client in (*3*)
+	
+  let authRequest = recieve client in (*3*)
 	match authRequest with
 	| SamlProtocolMessage (idp, message, sigSP, relay)-> 
-    (*assert (Log serviceprovider message);*)
+    
+    
+
     let challenge = CreateChallenge client in
+    assert (Log serviceprovider relay );
     let challengeMessage = Challenge challenge in
     send client challengeMessage; (*4*)
+    
     let credentials = recieve client in (*5*)
       match credentials with
       | Credentials(user, password, challenge') -> 
+  
         (*Check credentials and challenge*)
+  
         let (samlresponse, sigIDP) = CreateSamlResponse me serviceprovider Success in
         let response = SamlProtocolMessage serviceprovider samlresponse sigIDP relay in
         send client response(*6*)
+  
       | _ -> send client (Failed (400))(*6.3*)
-	| _ -> 
+	
+  | _ -> 
     let (samlresponse, sigIDP) = CreateSamlResponse me serviceprovider Requester in
     let response = SamlProtocolMessage serviceprovider samlresponse sigIDP relay in
-    send client response(*4.1*)
-  ()
+    send client response (*4.1*)
 
 end (*Identityprovider*)
